## User

Let \( n \) be an even positive integer. Let \( p \) be a monic, real polynomial of degree \( 2n \); that is to say,

\[
p(x) = x^{2n} + a_{2n-1}x^{2n-1} + \dots + a_1x + a_0
\]

for some real coefficients \( a_0, \dots, a_{2n-1} \).

Suppose that \( p\left( \frac{1}{k} \right) = k^2 \) for all integers \( k \) such that \( 1 \leq |k| \leq n \).

Find all other real numbers \( x \) for which \( p\left( \frac{1}{x} \right) = x^2 \).

## Assistant

### Chain of Thought

We are told that for all integer values of \( k \) satisfying \( 1 \leq |k| \leq n \), 
\[
p\left(\frac{1}{k}\right) = k^2
\]
Our problem is: Given that \( p \) is monic of degree \( 2n \), and that \( p\left(\frac{1}{k}\right) = k^2 \) for \( k = \pm1, \pm2, \dots, \pm n \), find all other real numbers \( x \) such that 
\[
p\left(\frac{1}{x}\right) = x^2.
\]

In other words, we are to find all real numbers \( x \) such that \( p\left(\frac{1}{x}\right) = x^2 \).

Firstly, note that:

- The monic polynomial \( p(z) \) is of degree \( 2n \).

- We have \( 2n \) data points: for \( k = \pm1 \text{ to } \pm n, p\left(\frac{1}{k}\right) = k^2 \).

But there are \( 2n \) distinct values of \( \frac{1}{k} \) (since \( k \) ranges over integers \( \pm1 \text{ to } \pm n \), and they are distinct).

Thus, we have \( 2n \) points \( (x, y) \) of the form \( \left( \frac{1}{k}, k^2 \right) \).

Thus, \( p \) is a polynomial of degree \( 2n \) that satisfies \( p\left(\frac{1}{k}\right) = k^2 \) for \( 2n \) values of \( \frac{1}{k} \).

Wait, but \( p\left(\frac{1}{x}\right) - x^2 = 0 \).

Our equation is \( p\left(\frac{1}{x}\right) - x^2 = 0 \).

Let me define \( q(x) = p\left(\frac{1}{x}\right) - x^2 \).

Our task is to find all real numbers \( x \) such that \( q(x) = 0 \).

Given the data from the problem, let’s consider that \( q(k) = p\left(\frac{1}{k}\right) - k^2 = 0 \) for \( k = \pm1, \pm2, \dots, \pm n \).

Thus, \( q(k) = 0 \) for \( k = \pm1, \dots, \pm n \).

Moreover, since \( p \) is a polynomial of degree \( 2n \), then \( p\left(\frac{1}{x}\right) \) is a rational function of \( x \) of degree \( 2n \) when considered as a function of \( x \).

But we can consider \( q(x) = p\left(\frac{1}{x}\right) - x^2 \).

Alternatively, let’s consider \( s(x) = x^{2n} p\left(\frac{1}{x}\right) - x^{2n+2} \).

Let me explain: We can consider that \( p\left(\frac{1}{x}\right) = x^{-2n} + a_{2n-1}x^{-2n+1} + \dots + a_0 \).

Then multiplying by \( x^{2n} \) gives:
\[
x^{2n} p\left(\frac{1}{x}\right) = 1 + a_{2n-1}x + a_{2n-2}x^2 + \dots + a_0 x^{2n}.
\]
Similarly, \( x^{2n+2} = x^{2n+2} \).

Thus, define the polynomial \( s(x) = x^{2n} p\left(\frac{1}{x}\right) - x^{2n+2} \).

But wait, perhaps it’s better to rearrange.

Let me consider that \( s(x) = x^{2n}\left[ p\left(\frac{1}{x}\right) - x^2 \right] = x^{2n} q(x) \).

So \( s(x) = x^{2n} q(x) \).

Since \( q(k) = 0 \) for \( k = \pm1, \dots, \pm n \), we have \( q(x) = 0 \).

Thus, \( q(x) = k^{2n} q(x) = 0 \).

Thus, \( q(k) = 0 \) at \( x = \pm1, \pm2, \dots, \pm n \).

Thus, \( s(x) \) is a polynomial (not a rational function), since \( x^{2n} q(x) \) is a polynomial.

Moreover, \( s(x) = x^{2n} \left[ p\left(\frac{1}{x}\right) - x^2 \right] = x^{2n} p\left(\frac{1}{x}\right) - x^{2n+2} \).

But \( x^{2n} p\left(\frac{1}{x}\right) = p^*(x) \).

Wait, but \( x^{2n} p\left(\frac{1}{x}\right) \) is the "reciprocal polynomial" of \( p(x) \), evaluated at \( x \).

But since \( p(x) \) is monic of degree \( 2n \), its reciprocal polynomial is monic of degree \( 2n \) as well.

Thus, set \( t(x) = x^{2n} p\left(\frac{1}{x}\right) \).

Let me write \( t(x) = x^{2n} p\left(\frac{1}{x}\right) = P^*(x) \).

\( P^*(x) \) is the reverse polynomial of \( p(x) \).

\( p(x) = x^{2n} + a_{2n-1}x^{2n-1} + \dots + a_0 \).

Then \( t(x) = x^{2n} p\left(\frac{1}{x}\right) = x^{2n} \left[ \frac{1}{x^{2n}} + a_{2n-1} \frac{1}{x^{2n-1}} + \dots + a_0 \right] = 1 + a_{2n-1} x + a_{2n-2} x^2 + \dots + a_0 x^{2n} \).

So \( t(x) = p^*(x) \), the reciprocal polynomial of \( p \).

Thus, \( s(x) = t(x) - x^{2n+2} = 1 + a_{2n-1}x + a_{2n-2}x^2 + \dots + a_0 x^{2n} - x^{2n+2} \).

But \( x^{2n+2} = x^{2n+2} \).

Therefore, \( s(x) = p^*(x) - x^{2n+2} \).

We can now write \( s(x) = p^*(x) - x^{2n+2} \).

Alternatively, \( p^*(x) - x^{2n+2} = s(x) \).

But \( t(x) = p^*(x) \), and \( s(x) = t(x) - x^{2n+2} \).

But our key is that \( s(x) = x^{2n} q(x) \).

Recall that \( q(k) = 0 \) for \( k = \pm1, \pm2, \dots, \pm n \).

Therefore, \( s(k) = 0 \) at \( x = \pm1, \dots, \pm n \).

Therefore, \( s(x) \) is a polynomial that vanishes at \( x = \pm1, \pm2, \dots, \pm n \).

\( s(x) \) has roots at \( x = \pm1, \dots, \pm n \).

Thus, \( s(x) \) must be divisible by the monic polynomial whose roots are at \( \pm1, \pm2, \dots, \pm n \).

Thus, \( s(x) = m(x)h(x) \).

Where \( m(x) = (x - (-n))(x - (-n + 1)) \dots (x - (2 - 1))(x - (1))(x - n) \).

Wait, that is, \( m(x) = \prod_{k=1}^n(x - k)(x + k) = \prod_{k=1}^n(x^2 - k^2) \).

Therefore, \( m(x) = \prod_{k=1}^n(x^2 - k^2) \).

Thus, \( m(x) \) is a monic polynomial of degree \( 2n \).

Similarly, since \( s(x) \) is of degree...

Let me compute the degree of \( s(x) \):

Since \( s(x) = x^{2n} p\left(\frac{1}{x}\right) - x^{2n+2} \), 

Compute \( t(x) = x^{2n} p\left(\frac{1}{x}\right) \).

We have \( p(z) = x^{2n} + a_{2n-1}x^{2n-1} + \dots + a_0 \).

Then \( t(x) = x^{2n} p\left(\frac{1}{x}\right) = x^{2n} \left[ \frac{1}{x^{2n}} + a_{2n-1}\frac{1}{x^{2n-1}} + \dots + a_0 \right] = 1 + a_{2n-1}x + a_{2n-2}x^2 + \dots + a_0 x^{2n} \).

So \( t(x) \) is a polynomial of degree \( 2n \).

What about \( x^{2n+2} \)?

So \( s(x) = t(x) - x^{2n+2} \).

Therefore, \( s(x) \) is a polynomial of degree \( \max(\text{degree of } t(x), \text{degree of } x^{2n+2}) = \text{degree of } x^{2n+2} \).

So \( s(x) \) is of degree \( 2n + 2 \).

But \( t(x) \) has degree \( 2n \).

So \( s(x) = [\text{degree } 2n \text{ polynomial}] - [\text{degree } (2n + 2) \text{ monomial}] = -x^{2n+2} + [\text{degree } \leq 2n \text{ polynomial}] \).

So the leading term of \( s(x) \) is \( -x^{2n+2} \).

Thus, \( s(x) \) is a polynomial of degree \( 2n + 2 \) with leading coefficient \( -1 \).

So \( s(x) = -x^{2n+2} + \text{lower degree terms} \).

Similarly, \( m(x) = \prod_{k=1}^n \left( x^2 - k^2 \right) = \text{monic polynomial of degree } 2n \).

Therefore, if we factor \( s(x) = m(x)h(x) \).

Since \( s(x) \) is degree \( 2n + 2 \) and \( m(x) \) is degree \( 2n \), \( h(x) \) must be degree 2.

Therefore, \( h(x) \) is a quadratic polynomial.

Our plan is to write \( s(x) = m(x)h(x) \).

Given that \( s(x) \) is degree \( 2n + 2 \) with leading coefficient \( -1 \).

Similarly, \( m(x) \) is a degree \( 2n \) monic polynomial.

Therefore, \( h(x) \) must be a degree 2 polynomial with leading coefficient \( -1 \).

Therefore, \( h(x) \) must be of the form \( h(x) = -x^2 + bx + c \).

Alternatively, since \( s(x) = m(x)h(x) \),

We can write \( s(x) = (-1)x^{2n+2} + [\text{lower degree terms}] \).

Also, \( m(x) = x^{2n} + [\text{lower degree terms}] \) (since it is monic of degree \( 2n \)).

Then \( s(x) = m(x)h(x) = \left[ x^{2n} + \dots \right](-x^2 + bx + c) = -x^{2n+2} + [\text{lower degree terms}] \).

Therefore, the leading term of \( s(x) \) is \( -x^{2n+2} \), which matches.

Therefore, our assertion that \( h(x) \) is degree 2 with leading coefficient \( -1 \) is consistent.

Therefore, \( h(x) = -x^2 + bx + c \).

Our task now is to find \( b \) and \( c \).

So we have:

\[
s(x) = m(x)h(x) = \left[ \prod_{k=1}^n (x^2 - k^2) \right] (-x^2 + bx + c)
\]

and

\[
s(x) = x^{2n} p\left(\frac{1}{x}\right) - x^{2n+2}.
\]

Equate the expressions for \( s(x) \).

Alternatively, let’s consider that \( t(x) = x^{2n} p\left(\frac{1}{x}\right) = p^*(x) \).

Then \( s(x) = t(x) - x^{2n+2} = p^*(x) - x^{2n+2} \).

Therefore, \( s(x) = m(x)h(x) \).

Thus, \( p^*(x) - x^{2n+2} = m(x)h(x) \).

But \( p^*(x) \) is degree \( 2n \) and \( x^{2n+2} \) is degree \( 2n + 2 \), so their difference is degree \( 2n + 2 \).

Therefore, the left-hand side \( p^*(x) - x^{2n+2} = [\text{degree} \leq 2n] - [\text{degree } 2n + 2] \).

Wait, but the \( x^{2n+2} \) term is of higher degree than \( p^*(x) \), so the leading term of \( s(x) \) is \( -x^{2n+2} \).

Similarly, the right-hand side \( m(x)h(x) = [\text{degree } 2n] \times [\text{degree } 2] = [\text{degree } 2n + 2] \).

Now, let’s write \( s(x) = -x^{2n+2} + \text{lower degree terms} \).

Similarly, \( m(x)h(x) = x^{2n}(-x^2 + bx + c) + \text{lower degree terms} \).

Compute \( m(x)h(x) = \left( x^{2n} + \text{lower degree terms} \right) (-x^2 + bx + c) \).

The product of \( x^{2n} \) and \( -x^2 \) gives \( -x^{2n+2} \).

Similarly, \( x^{2n} \cdot bx = bx^{2n+1} \).

And \( x^{2n} \cdot c = cx^{2n} \).

Thus, we find:

\[
s(x) = m(x)h(x) = -x^{2n+2} + bx^{2n+1} + cx^{2n} + \text{[lower degree terms]}.
\]

Similarly, \( s(x) = -x^{2n+2} + [\text{lower degree terms}] \).

Thus, to make the higher-degree terms match, \( s(x) = -x^{2n+2} + bx^{2n+1} + cx^{2n} + [\text{lower degree terms}] \).

Wait, but from the definition of \( s(x) \), we have:

\( s(x) = [t(x)] - x^{2n+2} = [\text{leading terms of } t(x)] - x^{2n+2} \).

But \( t(x) = p^*(x) = 1 + a_{2n-1}x + a_{2n-2}x^2 + \dots + a_0x^{2n} \).

Thus, \( t(x) = \) polynomial of degree \( \leq 2n \).

Therefore, \( s(x) = [\text{degree } \leq 2n] - x^{2n+2} = -x^{2n+2} + [\text{degree } \leq 2n] \).

Therefore, the highest degree term of \( s(x) \) is \( -x^{2n+2} \), and the rest is lower degree terms.

Therefore, \( s(x) = -x^{2n+2} + \text{lower degree terms} \).

So matching terms:

From \( m(x)h(x) \):

- Leading term of \( s(x) = -x^{2n+2} \)
- Second term: \( bx^{2n+1} \)
- Third term: \( cx^{2n} \)

But from \( s(x) = p^*(x) - x^{2n+2} \), and \( p(x) \) has degree \( \leq 2n \).

Therefore, there is no \( x^{2n+1} \) term in \( s(x) \) unless \( t(x) \) contributes, but \( t(x) \) is of degree \( \leq 2n \).

Given that \( s(x) = -x^{2n+2} + [\text{degree } \leq 2n] \),

Therefore, \( s(x) = -x^{2n+2} + bx^{2n+1} + a_{2n-1}x^{2n-1} + \dots + a_0 \).

Similarly, from the \( m(x)h(x) \) computation:

\[
s(x) = m(x)h(x) = \left[ x^{2n} + \dots \right](-x^2 + bx + c) = -x^{2n+2} + bx^{2n+1} + cx^{2n} + [\text{lower degree terms}]
\]

So from the above, the coefficient of \( x^{2n+1} \) in \( s(x) \) is \( b \).

But according to \( s(x) = -x^{2n+2} + [\text{degree } \leq 2n] \), the \( x^{2n+1} \) term is absent (since \( p^*(x) \) has degree \( \leq 2n \)).

Therefore, \( s(x) \) has no \( x^{2n+1} \) term.

Thus, the coefficient of \( x^{2n+1} \) in \( s(x) \) is zero.

Therefore, \( b = 0 \).

Similarly, let's now compare the coefficient of \( x^{2n} \) in \( s(x) \), which is \( cx^{2n} \).

Similarly, from \( s(x) = -x^{2n+2} + bx^{2n+1} + [\text{lower degree terms}] \),

So the coefficient of \( x^{2n} \) in \( s(x) \) is \( cx^{2n} = c \).

But \( s(x) = p^*(x) - x^{2n+2} \).

So \( s(x) = [p^*(x)] - x^{2n+2} \).

But \( p^*(x) \) has degree \( \leq 2n \).

Therefore, the \( 2n \) term in \( s(x) \) is given by the \( 2n \) term in \( p^*(x) \), which is \( a_0x^{2n} \).

So \( s(x) = (-x^{2n+2}) + a_0x^{2n} + [\text{lower degree terms}] \).

Therefore, comparing coefficients, the coefficient of \( x^{2n} \) in \( s(x) \) is \( a_0 \).

Thus, \( c = a_0 \).

So \( c = a_0 \).

So we have \( h(x) = -x^2 + c \).

But we already have \( b = 0 \).

Thus, \( h(x) = -x^2 + c \).

We can now write: \( s(x) = m(x)[-x^2 + c] = \left[ \prod_{k=1}^n (x^2 - k^2) \right] (-x^2 + c) \).

Similarly, \( s(x) = -x^{2n+2} + a_0x^{2n} + [\text{lower degree terms}] \).

We may be able to compute the expression \( m(x)[-x^2 + c] \) and match the coefficient of \( x^{2n} \).

Let me first consider \( m(x) = x^{2n} + [\text{lower degree terms}] \).

Similarly, \( m(x) \cdot (-x^2 + c) = -x^{2n+2} + cx^{2n} + [\text{lower degree terms}] \).

Therefore, \( s(x) = -x^{2n+2} + cx^{2n} + [\text{lower degree terms}] \).

But \( s(x) = -x^{2n+2} + a_0x^{2n} + [\text{lower degree terms}] \).

Therefore, \( c = a_0 \).

Therefore, \( c = a_0 \).

Thus, \( c = a_0 \).

So we’ve confirmed that \( c = a_0 \).

But what about the next term? Let’s consider matching the next coefficient.

Compute \( m(x) \cdot (-x^2 + c) = -x^{2n+2} + cx^{2n} + [\text{lower degree terms}] \).

The term of degree \( 2n - 2 \) in \( s(x) \) is due to the products:

- The \( x^{2n - 2} \) term from \( m(x) \) multiplied by \( -x^2 \).
- The \( x^{2n - 2} \) term from \( m(x) \) multiplied by \( c \).

Let me write \( m(x) = x^{2n} + m_{2n-2}x^{2n-2} + \text{lower terms} \).

Similarly, \( m(x) \cdot (-x^2) = (-x^{2n+2} + m_{2n-2}x^{2n} + \text{lower terms}) \).

Wait, actually, this may not help us directly without specific terms.

An alternative is to consider the known polynomials.

So \( m(x) = \prod_{k=1}^n (x^2 - k^2) \).

Similarly, \( s(x) = m(x)[-x^2 + c] \).

Now, consider that \( s(x) = [-x^{2n+2}] + cx^{2n} + [\text{lower degree terms}] \).

Similarly, expand \( m(x)[-x^2] \) and \( m(x) \cdot c \) separately.

Let me compute \( m(x) \cdot (-x^2) \).

Since \( m(x) \) is a monic degree \( 2n \) polynomial, its highest degree term is \( x^{2n} \).

Therefore, \( m(x) \cdot (-x^2) = -x^{2n+2} + \text{lower degree terms} \).

Similarly, \( m(x) \cdot c = cx^{2n} + \text{lower degree terms} \).

Therefore, \( s(x) = [-x^{2n+2}] + cx^{2n} + [\text{lower degree terms}] \).

Similarly, from the definition of \( s(x) \), \( s(x) = [-x^{2n+2}] + a_0x^{2n} + a_{2n-1}x^{2n-1} + \dots \).

But from \( a_0 = p^*(x) - x^{2n+2} \),

Since \( p^*(x) = 1 + a_{2n-1}x + a_{2n-2}x^2 + \dots + a_0x^{2n} \),

Thus, \( s(x) = [1 + a_{2n-1}x + a_{2n-2}x^2 + \dots + a_0x^{2n}] - x^{2n+2} \).

But this seems to contradict our prior assertion that \( s(x) = -x^{2n+2} + a_0x^{2n} + \dots \).

Wait, perhaps we need to be careful here.

Let me try to rewrite \( s(x) \).

Given that \( t(x) = p^*(x) = x^{2n}p\left(\frac{1}{x}\right) = 1 + a_{2n-1}x + \dots + a_0x^{2n} \),

Therefore, \( s(x) = t(x) - x^{2n+2} = [1 + a_{2n-1}x + \dots + a_0x^{2n}] - x^{2n+2} \).

So \( s(x) = -x^{2n+2} + a_0x^{2n} + [\text{lower degree terms}] \).

So the constant term of \( s(x) \) is \( s(0) = p^*(0) - 0 = p^*(0) = 1 \).

Similarly, \( m(x) \cdot h(x) \), when evaluated at \( x = 0 \), becomes \( m(0) \cdot h(0) = \left[ \prod_{k=1}^n (1 - k^2) \right] [-0 + c] = \left[ (-1)^n k_1^2 k_2^2 \dots k_n^2 \right] c \).

But since \( k = 1 \text{ to } n \), the product \( k^2 \) is

Wait, sorry, actually, \( \prod_{k=1}^n k^2 = (n!)^2 \)

So \( m(0) = (-1)^n(n!)^2 \).

Therefore, \( m(0)h(0) = (-1)^n(n!)^2(0 + c) = (-1)^n(n!)^2c \).

Similarly, \( s(0) = 1 \).

So we have:

\[
s(0) = m(0)h(0).
\]

\[
1 = (-1)^n(n!)^2c.
\]

Therefore,

\[
c = \frac{1}{(-1)^n(n!)^2} = (-1)^n \frac{1}{(n!)^2}.
\]

Wait, but \( c = a_0 \).

But we previously had \( c = a_0 \).

Therefore, \( a_0 = (-1)^n \frac{1}{(n!)^2} \).

But since \( c = a_0 \),

Thus, we have determined \( c \).

Similarly, perhaps we can find more about \( p^*(x) \).

But perhaps we can do better.

Alternatively, since \( p^*(x) = -x^{2n+2} = s(x) = m(x)h(x) \).

Given that \( m(x) = \prod_{k=1}^n (x^2 - k^2) = x^{2n} - (\text{sum of squares})x^{2n-2} + \dots + (-1)^n(n!)^2 \).

Similarly, \( t(x) = p^*(x) \).

Given \( p^*(x) = x^{2n} p\left( \frac{1}{x} \right) = x^{2n} \left(1 + a_{2n-1} \frac{1}{x} + a_{2n-2} \frac{1}{x^2} + \dots + a_0 \right) \).

Therefore, \( p^*(x) = 1 + a_{2n-1}x + a_{2n-2}x^2 + \dots + a_0 x^{2n} \).

Thus, \( p^*(x) \) is degree \( 2n \).

Similarly, \( s(x) = p^*(x) - x^{2n+2} \).

Now, what if we consider that \( p^*(x) = x^{2n+2} - m(x)h(x) \).

Wait, but that seems messy.

Alternatively, since \( s(x) = m(x)h(x) = [x^{2n} + \dots + (-1)^n(n!)^2](-x^2 + c) \).

To find \( p^*(x) \), we can write

\[
p^*(x) = x^{2n+2} - [m(x)x^2 + cm(x)] + x^{2n+2}.
\]

Thus, \( p^*(x) = [m(x)x^2 + cm(x)] + x^{2n+2} \).

Then, \( p^*(x) = [m(x)x^2 + cm(x)] + x^{2n+2} \).

So \( p^*(x) = [m(x)(-x^2 + c)] + x^{2n+2} \).

But \( x^{2n+2} = x^2x^{2n} \).

But \( m(x) \) is degree \( 2n \), and we can write \( x^{2n+2} = x^2a_0x^{2n} \).

So \( p^*(x) = m(x)x^2 + cm(x) + x^{2n+2} \).

But \( m(x)x^2 = a_2m(x) = x^{2n} + \dots \).

So let’s compute \( p^*(x) = -x^2m(x) + cm(x) + x^{2n+2} \).

But \( x^{2n+2} = x^2a_2 \), so:

\[
p^*(x) = -x^2m(x) + cm(x) + x^{2n+2}.
\]

Now \( m(x) \) is monic degree 2n: \( m(x) = x^{2n} + \dots + (-1)^n(n!)^2 \).

So \( 2x^2m(x) = x^{2n} + \text{lower degree terms} \).

Therefore, \( -x^2m(x) = -x^{2n+2} + \text{lower degree terms} \).

Similarly, \( a_2x^2 = x^{2n+2} \).

So \( p^*(x) = -x^2m(x) + cm(x) + x^{2n+2} = [-x^2m(x) + x^{2n}] + cm(x) \).

But \( x^2m(x) = x^{2n+2} + a_2m(x) \) (since \( m(0) \) is the leading coefficient of \( x^{2n} \), which is 1).

Therefore, \( -x^2m(x) + x^{2n+2} = -x^2[m(x) - x^{2n}] \).

But \( m(x) = x^{2n} + \text{lower degree terms} \).

Therefore, \( -x^2m(x) + x^{2n+2} = -x^2[m(x) - x^{2n}] \).

Thus, \( p^*(x) = -x^2[m(x) - x^{2n}] + cm(x) \).

Therefore, \( p^*(x) = -x^2[m(x) - x^{2n}] + cm(x) \). But \( m(x) - x^{2n} = \text{lower degree terms} \).

Similarly, \( p^*(x) = -x^2[\text{lower degree terms}] + cm(x) \).

So the term of degree \( 2n + 1 \) in \( p^*(x) \) comes from \( -x^2[m_{2n-1}x^{2n-1}] \) plus \( cm(x) \).

But \( p^*(x) \) has degree \( \leq 2n \).

Therefore, the degree of \( p^*(x) \) is \( \leq 2n \).

Similarly, the highest degree term in \( p^*(x) \) is \( x^{2n} \).

But from our prior expression, \( p^*(x) = -x^2[m(x) - x^{2n}] + cm(x) \).

But after simplification, the leading term is \( cx^{2n} \).

Wait, I think this is getting too messy.

Perhaps I should consider the concrete value of \( m(x) \) at \( x = 0 \).

We already considered

\[
s(0) = 1.
\]

Similarly, \( m(0) = (-1)^n(n!)^2 \).

Therefore, we established that \( 1 = s(0) = m(0)h(0) \).

But \( h(0) = 0 + c = c \).

So

\[
c = \frac{1}{m(0)} = \frac{1}{(-1)^n(n!)^2} = (-1)^n \frac{1}{(n!)^2}.
\]

So \( c = \frac{(-1)^n}{(n!)^2} \).

Similarly, we had \( c = a_0 \).

Therefore, \( a_0 = c = \frac{(-1)^n}{(n!)^2} \).

Therefore, the constant term in \( p^*(x) \) is \( p^*(0) = 1 \).

So we have \( p^*(0) = 1 \).

Similarly, \( s(0) = p^*(0) - 0 = 1 \).

So consistent.

But perhaps this is as far as we can go without specific computations.

Alternatively, the problem is to find all real numbers \( x \) satisfying

\[
p\left( \frac{1}{x} \right) = x^2.
\]

Given that \( p\left( \frac{1}{k} \right) = k^2 \) for \( k = \pm 1, \pm 2, \dots, \pm n \),

We might conjecture that the only real solutions are \( x = \pm (n+1), \pm (n+2), \dots \).

But since \( p\left( \frac{1}{x} \right) - x^2 = 0 \), and \( p\left( 1/k \right) \) is given, perhaps all solutions \( x \) satisfy \( p\left( 1/x \right) = x^2 \).

But we can express \( q(x) = p\left( 1/x \right) - x^2 \).

But \( q(x) \) has roots at \( x = \pm 1, \pm 2, \dots, \pm n \).

Similarly, the solutions we are looking for are zeros of \( q(x) \).

Thus, \( q(x) = \frac{s(x)}{x^2} \).

But \( s(x) = x^{2n}q(x) \).

Similarly, \( s(x) = m(x)h(x) \), where \( h(x) = -x^2 + c \).

So the zeros of \( q(x) \) are zeros of \( s(x) \) of degree \( 2n + 2 \) minus zeros at \( x = 0 \) multiplicity \( 2n \) (since \( s(x) = x^{2n}q(x) \)).

Therefore, zeros of \( q(x) \) are zeros of \( s(x) \), excluding \( x = 0 \).

Thus, zeros of \( q(x) \) are \( x = \pm 1, \dots, \pm n \), and zeros of \( h(x) \).

But \( h(x) = -x^2 + c = 0 \).

So the other zeros are solutions of \( -x^2 + c = 0 \).

So solving \( -x^2 + c = 0 \).

That is, \( x^2 = c \).

Thus, \( x = \pm \sqrt{c} \).

But \( c = \frac{(-1)^n}{(n!)^2} \).

So

\[
c = \frac{(-1)^n}{(n!)^2}.
\]

Therefore, \( c > 0 \) when \( n \) is even, since \( (-1)^n = 1 \).

Therefore, when \( n \) is even, \( c = \frac{1}{(n!)^2} > 0 \).

Thus, \( x^2 = c \) has real solutions \( x = \pm \sqrt{c} \).

Therefore, the other real solutions of \( p\left( \frac{1}{x} \right) = x^2 \) are \( x = \pm \sqrt{c} \).

Similarly, when \( n \) is even, \( c > 0 \).

Thus, the other real numbers \( x \) satisfying \( p\left( \frac{1}{x} \right) = x^2 \) are \( x = \pm \frac{1}{n+1} \).

Therefore, the other real numbers are \( x = \pm \frac{1}{n+1} \).

Wait, wait, \( x^2 = c \), so \( x = \pm \sqrt{\frac{1}{(n!)^2}} = \pm \frac{1}{n!} \).

Therefore, the other real numbers are \( x = \pm \frac{1}{n!} \).

So in conclusion, the numbers \( x \) satisfying \( p\left( \frac{1}{x} \right) = x^2 \) are \( x = \pm k \) for \( k = 1 \text{ to } n \), and \( x = \pm \frac{1}{n!} \).

Thus, the other real numbers are \( x = \pm \frac{1}{n!} \).

So the answer is \( x = \pm \frac{1}{n!} \) (along with \( x = \pm k \text{ for } k = 1 \text{ to } n \)).

Wait, but the problem says “Suppose that \( p\left( \frac{1}{k} \right) = k^2 \) for all integers \( k \) with \( 1 \leq |k| \leq n \). Find all other real numbers for which \( p\left( \frac{1}{x} \right) = x^2 \)."

Thus, apart from \( x = \pm k \) (which have already been given), the other real numbers are \( x = \pm \frac{1}{n!} \).

Wait, but when \( n \) is even, \( c = \frac{(-1)^n}{(n!)^2} = \frac{1}{(n!)^2} \).

Thus, \( c = \frac{1}{(n!)^2} \).

Thus, \( x^2 = c \Rightarrow x = \pm \frac{1}{n!} \).

Thus, the other real numbers are \( x = \pm \frac{1}{n!} \).

**Answer:** The other real numbers \( x \) satisfying \( p\left( \frac{1}{x} \right) = x^2 \) are \( x = \pm \frac{1}{n!} \).

### Answer

To solve this problem, we need to find all real numbers \( x \) such that

\[
p\left( \frac{1}{x} \right) = x^2,
\]

where \( p \) is a monic real polynomial of degree \( 2n \), and it is given that

\[
p\left( \frac{1}{k} \right) = k^2
\]

for all integers \( k \) with \( 1 \leq |k| \leq n \).

**Understanding the Given Information:**

1. **Given Data Points:** We have \( 2n \) data points from \( k = \pm 1, \pm 2, \dots, \pm n \), which provide the values \( p\left( \frac{1}{k} \right) = k^2 \).

2. **Polynomial Function:** \( p(x) \) is monic of degree \( 2n \), which means its highest-degree coefficient is 1.

**Defining a New Polynomial:**

Let's define a new function

\[
q(x) = p\left( \frac{1}{x} \right) - x^2.
\]

Our goal is to find all real solutions to \( q(x) = 0 \).

**Properties of \( q(x) \):**

- Since \( p \) is a polynomial of degree \( 2n \), \( p\left( \frac{1}{x} \right) \) can be expressed in powers of \( x \).
- The function \( q(x) \) has zeroes at \( x = \pm 1, \pm 2, \dots, \pm n \) because \( q(k) = p\left( \frac{1}{k} \right) - k^2 = 0 \).

**Constructing \( s(x) \):**

Consider the polynomial

\[
s(x) = x^{2n} q(x) = x^{2n} \left( p\left( \frac{1}{x} \right) - x^2 \right).
\]

Multiplying through by \( x^{2n} \) eliminates denominators, making \( s(x) \) a polynomial.

**Factoring \( s(x) \):**

We know that \( s(x) \) has roots at \( x = \pm 1, \pm 2, \dots, \pm n \). Therefore, \( s(x) \) can be expressed as:

\( s(x) = m(x)h(x) \),

where \( m(x) = \prod_{k=1}^n (x^2 - k^2) \) is a monic polynomial of degree \( 2n \) whose roots are \( \pm 1, \pm 2, \dots, \pm n \), and \( h(x) \) is a quadratic polynomial.

**Determining \( h(x) \):**

We consider \( h(x) \) to be a quadratic polynomial:

\[
h(x) = -x^2 + c,
\]

where \( c \) is a constant to be determined.

**Matching Coefficients:**

- The leading term of \( s(x) \) is \( -x^{2n+2} \).
- The leading term of \( m(x)h(x) \) is \( (x^{2n})(-x^2) = -x^{2n+2} \), ensuring the degrees match.

- **Comparing the constant term of \( s(x) \) using \( x = 0 \):**

\[
s(0) = p^*(0) - 0 = 1, \text{ where } p^*(x) = x^{2n} p\left( \frac{1}{x} \right).
\]

- **Evaluating \( m(0) \) and \( h(0) \):**

\[
m(0) = (-1)^n(n!)^2.
\]

\[
h(0) = -0 + c = c.
\]

- Since \( s(0) = m(0)h(0) \):

\[
1 = (-1)^n (n!)^2 c,
\]

which gives:

\[
c = \frac{1}{(-1)^n(n!)^2} = \frac{(-1)^n}{(n!)^2}.
\]

- For \( n \) even (since \( n \) is even), \( (-1)^n = 1 \), so \( c > 0 \).

**Finding Additional Solutions:**

Solving \( h(x) = 0 \):

\[
-x^2 + c = 0 \Rightarrow x^2 = c \Rightarrow x = \pm \frac{1}{n!},
\]

since \( c = \frac{1}{(n!)^2} \).

**Conclusion:**

The additional real numbers \( x \) satisfying \( p\left( \frac{1}{x} \right) = x^2 \) are \( x = \pm \frac{1}{n!} \).
